src/Inflist.v
@@ -1,0 +1,53 @@
+Require Import List.
+Import ListNotations.
+Require Import Coq.Arith.PeanoNat.
+
+(* Borrow from CompCert *)
+Require Import Coqlib.
+Require Import Integers.
+
+Require Import AST.
+
+Import HaskellListNotations.
+Open Scope string_scope.
+
+Definition inflist := (NonRecursive
+                         (Decl 245 (DExpr
+                                      (EApp (EApp
+                                               (ETApp (EVar 52) (TCon (TC (TCNum 8)) []))
+                                               (ETApp (ETApp (EVar 0) (TCon (TC (TCNum 1)) [])) (TCon (TC (TCNum 8)) [])))
+                                            (ETApp (ETApp (EVar 0) (TCon (TC (TCNum 2)) [])) (TCon (TC (TCNum 8)) [])))))).
+
+Definition finlist := (NonRecursive (Decl 246 (DExpr (EList [(ETApp (ETApp (EVar 0) (TCon (TC (TCNum 1)) [])) (TCon (TC (TCNum 8)) [])),(ETApp (ETApp (EVar 0) (TCon (TC (TCNum 2)) [])) (TCon (TC (TCNum 8)) [])),(ETApp (ETApp (EVar 0) (TCon (TC (TCNum 3)) [])) (TCon (TC (TCNum 8)) []))])))).
+
+Definition elem := (NonRecursive (Decl 247 (DExpr (EApp (EApp (ETApp (ETApp (ETApp (EVar 40) (TCon (TC (TCNum 3)) [])) (TCon (TC TCSeq) [TCon (TC (TCNum 8)) [],TCon (TC TCBit) []])) (TCon (TC (TCNum 1)) [])) (EVar 246)) (ETApp (ETApp (EVar 0) (TCon (TC (TCNum 1)) [])) (TCon (TC (TCNum 1)) [])))))).
+
+Definition rec := (NonRecursive (Decl 246 (DExpr (ERec [("x",(ETApp (ETApp (EVar 0) (TCon (TC (TCNum 3)) [])) (TCon (TC (TCNum 8)) []))),("y",(ETApp (ETApp (EVar 0) (TCon (TC (TCNum 5)) [])) (TCon (TC (TCNum 8)) [])))])))).
+
+Definition rec_select := (NonRecursive (Decl 247 (DExpr (ESel (EVar 246) (RecordSel "x"))))).
+
+Definition rec_ge := bind_decl_group rec (bind_decl_group rec_select gempty).
+
+Lemma nz :
+  8%nat <> 0%nat.
+Proof.
+  congruence.
+Qed.
+
+Lemma rec_eval :
+  eval_expr rec_ge empty (EVar 247) (bits (@repr 8 nz 3)).
+Proof.
+  eapply eval_global_var. reflexivity. unfold rec_ge.
+  simpl. reflexivity.
+  econstructor. eapply eval_global_var. reflexivity.
+  unfold rec_ge. simpl. reflexivity.
+  econstructor. simpl.
+  repeat econstructor.
+  simpl. unfold zrepr.
+  f_equal. f_equal.
+  match goal with
+  | [ |- ?X = ?Y ] => destruct (@eq_spec _ nz X Y); try congruence
+  end.
+  Unshelve.
+  all: omega.
+Qed.
